wormhole/aggregator/src/layer1/circuit/mod.rs
@@ -1,6 +1,0 @@
-pub mod build;
-pub mod circuit_logic;
-pub mod constants;
-
-pub use build::generate_layer1_circuit_binaries;
-pub use circuit_logic::{Layer1AggregationCircuit, Layer1AggregationCircuitTargets};
